Replace type_term by inductive

src/Typing_Defs.thy
@@ -2,45 +2,38 @@ theory Typing_Defs
   imports Set_Semantics
 begin
 
-fun type_term :: "('a \<Rightarrow> nat) \<Rightarrow> 'a pset_term \<Rightarrow> nat option" where
-    "type_term _ (\<emptyset> n) = Some (Suc n)"
-  | "type_term v (Var x) = Some (v x)"
-  | "type_term v (Single t) = map_option Suc (type_term v t)"
-  | "type_term v (s \<squnion>\<^sub>s t) = do {
-                              ts <- type_term v s;
-                              tt <- type_term v t;
-                              if ts = tt \<and> ts \<noteq> 0 then Some ts else None
-                            }"
-  | "type_term v (s \<sqinter>\<^sub>s t) = do {
-                              ts <- type_term v s;
-                              tt <- type_term v t;
-                              if ts = tt \<and> ts \<noteq> 0 then Some ts else None
-                            }"
-  | "type_term v (s -\<^sub>s t) = do {
-                              ts <- type_term v s;
-                              tt <- type_term v t;
-                              if ts = tt \<and> ts \<noteq> 0 then Some ts else None
-                            }"
+inductive types_pset_term :: "('a \<Rightarrow> nat) \<Rightarrow> 'a pset_term \<Rightarrow> nat \<Rightarrow> bool" ("_ \<turnstile> _ : _" 45) where
+  "v \<turnstile> \<emptyset> n : Suc n"
+| "v \<turnstile> Var x : v x"
+| "v \<turnstile> t : l \<Longrightarrow> v \<turnstile> Single t : Suc l"
+| "v \<turnstile> s : l \<Longrightarrow> v \<turnstile> t : l \<Longrightarrow> l \<noteq> 0 \<Longrightarrow> v \<turnstile> s \<squnion>\<^sub>s t : l"
+| "v \<turnstile> s : l \<Longrightarrow> v \<turnstile> t : l \<Longrightarrow> l \<noteq> 0 \<Longrightarrow> v \<turnstile> s \<sqinter>\<^sub>s t : l"
+| "v \<turnstile> s : l \<Longrightarrow> v \<turnstile> t : l \<Longrightarrow> l \<noteq> 0 \<Longrightarrow> v \<turnstile> s -\<^sub>s t : l"
 
-declare type_term.simps[simp del]
+inductive_cases types_pset_term_cases:
+  "v \<turnstile> \<emptyset> n : l" "v \<turnstile> Var x : l" "v \<turnstile> Single t : l"
+  "v \<turnstile> s \<squnion>\<^sub>s t : l" "v \<turnstile> s \<sqinter>\<^sub>s t : l" "v \<turnstile> s -\<^sub>s t : l"
 
-consts types :: "('a \<Rightarrow> nat) \<Rightarrow> 'b \<Rightarrow> bool" (infix "\<turnstile>" 45)
+lemma types_pset_term_intros':
+  "l = Suc n \<Longrightarrow> v \<turnstile> \<emptyset> n : l"
+  "l = v x \<Longrightarrow> v \<turnstile> Var x : l"
+  "l \<noteq> 0 \<Longrightarrow> v \<turnstile> t : nat.pred l \<Longrightarrow> v \<turnstile> Single t : l"
+  by (auto simp add: types_pset_term.intros(1,2,3) pred_def split: nat.splits)
 
-inductive types_pset_atom :: "('a \<Rightarrow> nat) \<Rightarrow> 'a pset_atom \<Rightarrow> bool" where
-  "\<lbrakk> type_term v s = Some l; type_term v t = Some l \<rbrakk> \<Longrightarrow> types_pset_atom v (s =\<^sub>s t)"
-| "\<lbrakk> type_term v s = Some l; type_term v t = Some (Suc l)\<rbrakk> \<Longrightarrow> types_pset_atom v (s \<in>\<^sub>s t)"
+definition type_of_term :: "('a \<Rightarrow> nat) \<Rightarrow> 'a pset_term \<Rightarrow> nat" where
+  "type_of_term v t \<equiv> THE l. v \<turnstile> t : l"
 
-adhoc_overloading types types_pset_atom
+inductive types_pset_atom :: "('a \<Rightarrow> nat) \<Rightarrow> 'a pset_atom \<Rightarrow> bool" (infix "\<turnstile>" 45) where
+  "\<lbrakk> v \<turnstile> s : l; v \<turnstile> t : l \<rbrakk> \<Longrightarrow> v \<turnstile> s =\<^sub>s t"
+| "\<lbrakk> v \<turnstile> s : l; v \<turnstile> t : Suc l\<rbrakk> \<Longrightarrow> v \<turnstile> s \<in>\<^sub>s t"
 
 inductive_cases types_pset_atom_Member_cases:
   "v \<turnstile> s \<in>\<^sub>s t1 \<squnion>\<^sub>s t2" "v \<turnstile> s \<in>\<^sub>s t1 \<sqinter>\<^sub>s t2" "v \<turnstile> s \<in>\<^sub>s t1 -\<^sub>s t2" "v \<turnstile> s \<in>\<^sub>s Single t"
 
-definition types_pset_fm :: "('a \<Rightarrow> nat) \<Rightarrow> 'a pset_fm \<Rightarrow> bool" where
+definition types_pset_fm :: "('a \<Rightarrow> nat) \<Rightarrow> 'a pset_fm \<Rightarrow> bool" (infix "\<turnstile>" 45) where
   "types_pset_fm v \<phi> \<equiv> (\<forall>a \<in> atoms \<phi>. v \<turnstile> a)"
 
-adhoc_overloading types types_pset_fm
-
-abbreviation "urelem' v (\<phi> :: 'a pset_fm) t \<equiv> v \<turnstile> \<phi> \<and> type_term v t = Some 0"
+abbreviation "urelem' v (\<phi> :: 'a pset_fm) t \<equiv> v \<turnstile> \<phi> \<and> v \<turnstile> t : 0"
 
 definition urelem :: "'a pset_fm \<Rightarrow> 'a pset_term \<Rightarrow> bool" where
   "urelem \<phi> t \<equiv> (\<exists>v. urelem' v \<phi> t)"
